\documentclass{article}
\usepackage{amsmath}
\usepackage{amssymb}

\begin{document}

\begin{align*}
U(x,y) &= y \left[ -2 \frac{\ln(\cosh x)}{x^2} + \frac{x - \tanh x}{x^2} y + \frac{\tanh x}{x} (2 - y \tanh x) \right] \\
       &= y \left[ 1 + \frac{2}{9} x^4 - \left( \frac{2}{3} x - \frac{8}{15} x^3 \right) y \right] + [5]
\end{align*}

\begin{align*}
V(x,y) &= 2 \frac{\ln(\cosh x)}{x} + 2 \frac{\tanh x - x}{x} y \\
       &= x \left[ 1 - \frac{1}{3} x^2 - \left( \frac{2}{3} x - \frac{4}{15} x^3 \right) y \right] + [5]
\end{align*}

\end{document}