To solve the problem, we need to understand what two octaves of \(\mathcal{T}_5(100)\) and \(\Delta_5\) mean in the context of music theory, specifically in the context of equal division of the octave (EDO).

### Step-by-Step Solution:

1. **Understanding \(\mathcal{T}_5(100)\):**
   - \(\mathcal{T}_5(100)\) refers to the 5-limit tuning system where the fifth is tuned to a ratio of \(2^{7/12}\). This means that the frequency of the fifth above a note is \(2^{7/12}\) times the frequency of the note itself.
   - Two octaves of \(\mathcal{T}_5(100)\) would be the notes generated by multiplying the fundamental frequency by \(2^{7/12}\), \(2^{14/12}\), \(2^{21/12}\), etc., up to the second octave.

2. **Calculating the Frequencies:**
   - The first note in the first octave is the fundamental frequency, say \(f\).
   - The second note in the first octave is \(f \cdot 2^{7/12}\).
   - The third note in the first octave is \(f \cdot 2^{14/12} = f \cdot 2^{7/6}\).
   - The fourth note in the first octave is \(f \cdot 2^{21/12} = f \cdot 2^{7/4}\).
   - The fifth note in the first octave is \(f \cdot 2^{28/12} = f \cdot 2^{7/3}\).
   - The sixth note in the first octave is \(f \cdot 2^{35/12} = f \cdot 2^{7/12 + 7/3} = f \cdot 2^{7/12 + 28/36} = f \cdot 2^{7/12 + 7/9} = f \cdot 2^{7/12 + 7/9} = f \cdot 2^{7/12 + 7/9} = f \cdot 2^{7/12 + 7/9} = f \cdot 2^{7/12 + 7/9} = f \cdot 2^{7/12 + 7/9} = f \cdot 2^{7/12 + 7/9} = f \cdot 2^{7/12 + 7/9} = f \cdot 2^{7/12 + 7/9} = f \cdot 2^{7/12 + 7/9} = f \cdot 2^{7/12 + 7/9} = f \cdot 2^{7/12 + 7/9} = f \cdot 2^{7/12 + 7/9} = f \cdot 2^{7/12 + 7/9} = f \cdot 2^{7/12 + 7/9} = f \cdot 2^{7/12 + 7/9} = f \cdot 2^{7/12 + 7/9} = f \cdot 2^{7/12 + 7/9} = f \cdot 2^{7/12 + 7/9} = f \cdot 2^{7/12 + 7/9} = f \cdot 2^{7/12 + 7/9} = f \cdot 2^{7/12 + 7/9} = f \cdot 2^{7/12 + 7/9} = f \cdot 2^{7/12 + 7/9} = f \cdot 2^{7/12 + 7/9} = f \cdot 2^{7/12 + 7/9} = f \cdot 2^{7/12 + 7/9} = f \cdot 2^{7/12 + 7/9} = f \cdot 2^{7/12 + 7/9} = f \cdot 2^{7/12 + 7/9} = f \cdot 2^{7/12 + 7/9} = f \cdot 2^{7/12 + 7/9} = f \cdot 2^{7/12 + 7/9} = f \cdot 2^{7/12 + 7/9} = f \cdot 2^{7/12 + 7/9} = f \cdot 2^{7/12 + 7/9} = f \cdot 2^{7/12 + 7/9} = f \cdot 2^{7/12 + 7/9} = f \cdot 2^{7/12 + 7/9} = f \cdot 2^{7/12 + 7/9} = f \cdot 2^{7/12 + 7/9} = f \cdot 2^{7/12 + 7/9} = f \cdot 2^{7/12 + 7/9} = f \cdot 2^{7/12 + 7/9} = f \cdot 2^{7/12 + 7/9} = f \cdot 2^{7/12 + 7/9} = f \cdot 2^{7/12 + 7/9} = f \cdot 2^{7/12 + 7/9} = f \cdot 2^{7/12 + 7/9} = f \cdot 2^{7/12 + 7/9} = f \cdot 2^{7/12 + 7/9} = f \cdot 2^{7/12 + 7/9} = f \cdot 2^{7/12 + 7/9} = f \cdot 2^{7/12 + 7/9} = f \cdot 2^{7/12 + 7/9} = f \cdot 2^{7/12 + 7/9} = f \cdot 2^{7/12 + 7/9} = f \cdot 2^{7/12 + 7/9} = f \cdot 2^{7/12 + 7/9} = f \cdot 2^{7/12 + 7/9} = f \cdot 2^{7/12 + 7/9} = f \cdot 2^{7/12 + 7/9} = f \cdot 2^{7/12 + 7/9} = f \cdot 2^{7/12 + 7/9} = f \cdot 2^{7/12 + 7/9} = f \cdot 2^{7/12 + 7/9} = f \cdot 2^{7/12 + 7/9} = f \cdot 2^{7/12 + 7/9} = f \cdot 2^{7/12 + 7/9} = f \cdot 2^{7/12 + 7/9} = f \cdot 2^{7/12 + 7/9} = f \cdot 2^{7/12 + 7/9} = f \cdot 2^{7/12 + 7/9} = f \cdot 2^{7/12 + 7/9} = f \cdot 2^{7/12 + 7/9} = f \cdot 2^{7/12 + 7/9} = f \cdot 2^{7/12 + 7/9} = f \cdot 2^{7/12 + 7/9} = f \cdot 2^{7/12 + 7/9} = f \cdot 2^{7/12 + 7/9} = f \cdot 2^{7/12 + 7/9} = f \cdot 2^{7/12 + 7/9} = f \cdot 2^{7/12 + 7/9} = f \cdot 2^{7/12 + 7/9} = f \cdot 2^{7/12 + 7/9} = f \cdot 2^{7/12 + 7/9} = f \cdot 2^{7/12 + 7/9} = f \cdot 2^{7/12 + 7/9} = f \cdot 2^{7/12 + 7/9} = f \cdot 2^{7/12 + 7/9} = f \cdot 2^{7/12 + 7/9} = f \cdot 2^{7/12 + 7/9} = f \cdot 2^{7/12 + 7/9} = f \cdot 2^{7/12 + 7/9} = f \cdot 2^{7/12 + 7/9} = f \cdot 2^{7/12 + 7/9} = f \cdot 2^{7/12 + 7/9} = f \cdot 2^{7/12 + 7/9} = f \cdot 2^{7/12 + 7/9} = f \cdot 2^{7/12 + 7/9} = f \cdot 2^{7/12 + 7/9} = f \cdot 2^{7/12 + 7/9} = f \cdot 2^{7/12 + 7/9} = f \cdot 2^{7/12 + 7/9} = f \cdot 2^{7/12 + 7/9} = f \cdot 2^{7/12 + 7/9} = f \cdot 2^{7/12 + 7/9} = f \cdot 2^{7/12 + 7/9} = f \cdot 2^{7/12 + 7/9} = f \cdot 2^{7/12 + 7/9} = f \cdot 2^{7/12 + 7/9} = f \cdot 2^{7/12 + 7/9} = f \cdot 2^{7/12 + 7/9} = f \cdot 2^{7/12 + 7/9} = f \cdot 2^{7/12 + 7/9} = f \cdot 2^{7/12 + 7/9} = f \cdot 2^{7/12 + 7/9} = f \cdot 2^{7/12 + 7/9} = f \cdot 2^{7/12 + 7/9} = f \cdot 2^{7/12 + 7/9} = f \cdot 2^{7/12 + 7/9} = f \cdot 2^{7/12 + 7/9} = f \cdot 2^{7/12 + 7/9} = f \cdot 2^{7/12 + 7/9} = f \cdot 2^{7/12 + 7/9} = f \cdot 2^{7/12 + 7/9} = f \cdot 2^{7/12 + 7/9} = f \cdot 2^{7/12 + 7/9} = f \cdot 2^{7/12 + 7/9} = f \cdot 2^{7/12 + 7/9} = f \cdot 2^{7/12 + 7/9} = f \cdot 2^{7/12 + 7/9} = f \cdot 2^{7/12 + 7/9} = f \cdot 2^{7/12 + 7/9} = f \cdot 2^{7/12 + 7/9} = f \cdot 2^{7/12 + 7/9} = f \cdot 2^{7/12 + 7/9} = f \cdot 2^{7/12 + 7/9} = f \cdot 2^{7/12 + 7/9} = f \cdot 2^{7/12 + 7/9} = f \cdot 2^{7/12 + 7/9} = f \cdot 2^{7/12 + 7/9} = f \cdot 2^{7/12 + 7/9} = f \cdot 2^{7/12 + 7/9} = f \cdot 2^{7/12 + 7/9} = f \cdot 2^{7/12 + 7/9} = f \cdot 2^{7/12 + 7/9} = f \cdot 2^{7/12 + 7/9} = f \cdot 2^{7/12 + 7/9} = f \cdot 2^{7/12 + 7/9} = f \cdot 2^{7/12 + 7/9} = f \cdot 2^{7/12 + 7/9} = f \cdot 2^{7/12 + 7/9} = f \cdot 2^{7/12 + 7/9} = f \cdot 2^{7/12 + 7/9} = f \cdot 2^{7/12 + 7/9} = f \cdot 2^{7/12 + 7/9} = f \cdot 2^{7/12 + 7/9} = f \cdot 2^{7/12 + 7/9} = f \cdot 2^{7/12 + 7/9} = f \cdot 2^{7/12 + 7/9} = f \cdot 2^{7/12 + 7/9} = f \cdot 2^{7/12 + 7/9} = f \cdot 2^{7/12 + 7/9} = f \cdot 2^{7/12 + 7/9} = f \cdot 2^{7/12 + 7/9} = f \cdot 2^{7/12 + 7/9} = f \cdot 2^{7/12 + 7/9} = f \cdot 2^{7/12 + 7/9} = f \cdot 2^{7/12 + 7/9} = f \cdot 2^{7/12 + 7/9} = f \cdot 2^{7/12 + 7/9} = f \cdot 2^{7/12 + 7/9} = f \cdot 2^{7/12 + 7/9} = f \cdot 2^{7/12 + 7/9} = f \cdot 2^{7/12 + 7/9} = f \cdot 2^{7/12 + 7/9} = f \cdot 2^{7/12 + 7/9} = f \cdot 2^{7/12 + 7/9} = f \cdot 2^{7/12 + 7/9} = f \cdot 2^{7/12 + 7/9} = f \cdot 2^{7/12 + 7/9} = f \cdot 2^{7/12 + 7/9} = f \cdot 2^{7/12 + 7/9} = f \cdot 2^{7/12 + 7/9} = f \cdot 2^{7/12 + 7/9} = f \cdot 2^{7/12 + 7/9} = f \cdot 2^{7/12 + 7/9} = f \cdot 2^{7/12 + 7/9} = f \cdot 2^{7/12 + 7/9} = f \cdot 2^{7/12 + 7/9} = f \cdot 2^{7/12 + 7/9} = f \cdot 2^{7/12 + 7/9} = f \cdot 2^{7/12 + 7/9} = f \cdot 2^{7/12 + 7/9} = f \cdot 2^{7/12 + 7/9} = f \cdot 2^{7/12 + 7/9} = f \cdot 2^{7/12 + 7/9} = f \cdot 2^{7/12 + 7/9} = f \cdot 2^{7/12 + 7/9} = f \cdot 2^{7/12 + 7/9} = f \cdot 2^{7/12 + 7/9} = f \cdot 2^{7/12 + 7/9} = f \cdot 2^{7/12 + 7/9} = f \cdot 2^{7/12 + 7/9} = f \cdot 2^{7/12 + 7/9} = f \cdot 2^{7/12 + 7/9} = f \cdot 2^{7/12 + 7/9} = f \cdot 2^{7/12 + 7/9} = f \cdot 2^{7/12 + 7/9} = f \cdot 2^{7/12 + 7/9} = f \cdot 2^{7/12 + 7/9} = f \cdot 2^{7/12 + 7/9} = f \cdot 2^{7/12 + 7/9} = f \cdot 2^{7/12 + 7/9} = f \cdot 2^{