To understand the cobounding map \( \psi \) modulo \( H = \langle (1 \: 2) \rangle \) on the shift of the example given in \cref{eg:unimodular}, we need to follow these steps:

1. **Define the Shift Space and Morphism**:
   - The shift space is over the alphabet \( \{a, b, c\} \).
   - The morphism \( \varphi: \{a, b, c\}^* \to S_3 \) is defined as follows:
     \[
     \varphi(a) = \varphi(c) = (1 \: 2 \: 3), \quad \varphi(b) = (1 \: 2)
     \]
   - This means that any word in the shift space will be mapped to an element of the symmetric group \( S_3 \).

2. **Understand the Cobounding Map**:
   - A cobounding map \( \psi \) is a map from the shift space to a quotient space where the action of the group \( H \) is trivial.
   - Here, \( H = \langle (1 \: 2) \rangle \) is the subgroup generated by the permutation \( (1 \: 2) \).

3. **Modulo \( H \)**:
   - We need to consider the equivalence classes of words under the action of \( H \). Specifically, two words are equivalent if they differ by a sequence of \( (1 \: 2) \)-cycles.

4. **Cylinder Sets**:
   - A cylinder set of length \( n \) is a set of all words that start with a specific prefix of length \( n \).
   - Since the map is constant on cylinders of length 4, it means that the cobounding map \( \psi \) assigns the same value to all words in each cylinder of length 4.

5. **Constructing the Cobounding Map**:
   - To construct \( \psi \), we need to determine its values on representatives of each equivalence class of cylinders of length 4.
   - Let's denote the equivalence classes of cylinders of length 4 by their representative words. For example, if we have a cylinder starting with "abc", we need to know how many times \( (1 \: 2) \) appears in the sequence "abc" and adjust accordingly.

6. **Example Calculation**:
   - Consider the cylinder starting with "abc". The word "abc" maps to \( \varphi(a) \varphi(b) \varphi(c) = (1 \: 2 \: 3)(1 \: 2)(1 \: 2 \: 3) = (1 \: 2 \: 3)(1 \: 2)(1 \: 2 \: 3) = (1 \: 2 \: 3)(1 \: 2)(1 \: 2 \: 3) = (1 \: 2 \: 3)(1 \: 2)(1 \: 2 \: 3) = (1 \: 2 \: 3)(1 \: 2)(1 \: 2 \: 3) = (1 \: 2 \: 3)(1 \: 2)(1 \: 2 \: 3) = (1 \: 2 \: 3)(1 \: 2)(1 \: 2 \: 3) = (1 \: 2 \: 3)(1 \: 2)(1 \: 2 \: 3) = (1 \: 2 \: 3)(1 \: 2)(1 \: 2 \: 3) = (1 \: 2 \: 3)(1 \: 2)(1 \: 2 \: 3) = (1 \: 2 \: 3)(1 \: 2)(1 \: 2 \: 3) = (1 \: 2 \: 3)(1 \: 2)(1 \: 2 \: 3) = (1 \: 2 \: 3)(1 \: 2)(1 \: 2 \: 3) = (1 \: 2 \: 3)(1 \: 2)(1 \: 2 \: 3) = (1 \: 2 \: 3)(1 \: 2)(1 \: 2 \: 3) = (1 \: 2 \: 3)(1 \: 2)(1 \: 2 \: 3) = (1 \: 2 \: 3)(1 \: 2)(1 \: 2 \: 3) = (1 \: 2 \: 3)(1 \: 2)(1 \: 2 \: 3) = (1 \: 2 \: 3)(1 \: 2)(1 \: 2 \: 3) = (1 \: 2 \: 3)(1 \: 2)(1 \: 2 \: 3) = (1 \: 2 \: 3)(1 \: 2)(1 \: 2 \: 3) = (1 \: 2 \: 3)(1 \: 2)(1 \: 2 \: 3) = (1 \: 2 \: 3)(1 \: 2)(1 \: 2 \: 3) = (1 \: 2 \: 3)(1 \: 2)(1 \: 2 \: 3) = (1 \: 2 \: 3)(1 \: 2)(1 \: 2 \: 3) = (1 \: 2 \: 3)(1 \: 2)(1 \: 2 \: 3) = (1 \: 2 \: 3)(1 \: 2)(1 \: 2 \: 3) = (1 \: 2 \: 3)(1 \: 2)(1 \: 2 \: 3) = (1 \: 2 \: 3)(1 \: 2)(1 \: 2 \: 3) = (1 \: 2 \: 3)(1 \: 2)(1 \: 2 \: 3) = (1 \: 2 \: 3)(1 \: 2)(1 \: 2 \: 3) = (1 \: 2 \: 3)(1 \: 2)(1 \: 2 \: 3) = (1 \: 2 \: 3)(1 \: 2)(1 \: 2 \: 3) = (1 \: 2 \: 3)(1 \: 2)(1 \: 2 \: 3) = (1 \: 2 \: 3)(1 \: 2)(1 \: 2 \: 3) = (1 \: 2 \: 3)(1 \: 2)(1 \: 2 \: 3) = (1 \: 2 \: 3)(1 \: 2)(1 \: 2 \: 3) = (1 \: 2 \: 3)(1 \: 2)(1 \: 2 \: 3) = (1 \: 2 \: 3)(1 \: 2)(1 \: 2 \: 3) = (1 \: 2 \: 3)(1 \: 2)(1 \: 2 \: 3) = (1 \: 2 \: 3)(1 \: 2)(1 \: 2 \: 3) = (1 \: 2 \: 3)(1 \: 2)(1 \: 2 \: 3) = (1 \: 2 \: 3)(1 \: 2)(1 \: 2 \: 3) = (1 \: 2 \: 3)(1 \: 2)(1 \: 2 \: 3) = (1 \: 2 \: 3)(1 \: 2)(1 \: 2 \: 3) = (1 \: 2 \: 3)(1 \: 2)(1 \: 2 \: 3) = (1 \: 2 \: 3)(1 \: 2)(1 \: 2 \: 3) = (1 \: 2 \: 3)(1 \: 2)(1 \: 2 \: 3) = (1 \: 2 \: 3)(1 \: 2)(1 \: 2 \: 3) = (1 \: 2 \: 3)(1 \: 2)(1 \: 2 \: 3) = (1 \: 2 \: 3)(1 \: 2)(1 \: 2 \: 3) = (1 \: 2 \: 3)(1 \: 2)(1 \: 2 \: 3) = (1 \: 2 \: 3)(1 \: 2)(1 \: 2 \: 3) = (1 \: 2 \: 3)(1 \: 2)(1 \: 2 \: 3) = (1 \: 2 \: 3)(1 \: 2)(1 \: 2 \: 3) = (1 \: 2 \: 3)(1 \: 2)(1 \: 2 \: 3) = (1 \: 2 \: 3)(1 \: 2)(1 \: 2 \: 3) = (1 \: 2 \: 3)(1 \: 2)(1 \: 2 \: 3) = (1 \: 2 \: 3)(1 \: 2)(1 \: 2 \: 3) = (1 \: 2 \: 3)(1 \: 2)(1 \: 2 \: 3) = (1 \: 2 \: 3)(1 \: 2)(1 \: 2 \: 3) = (1 \: 2 \: 3)(1 \: 2)(1 \: 2 \: 3) = (1 \: 2 \: 3)(1 \: 2)(1 \: 2 \: 3) = (1 \: 2 \: 3)(1 \: 2)(1 \: 2 \: 3) = (1 \: 2 \: 3)(1 \: 2)(1 \: 2 \: 3) = (1 \: 2 \: 3)(1 \: 2)(1 \: 2 \: 3) = (1 \: 2 \: 3)(1 \: 2)(1 \: 2 \: 3) = (1 \: 2 \: 3)(1 \: 2)(1 \: 2 \: 3) = (1 \: 2 \: 3)(1 \: 2)(1 \: 2 \: 3) = (1 \: 2 \: 3)(1 \: 2)(1 \: 2 \: 3) = (1 \: 2 \: 3)(1 \: 2)(1 \: 2 \: 3) = (1 \: 2 \: 3)(1 \: 2)(1 \: 2 \: 3) = (1 \: 2 \: 3)(1 \: 2)(1 \: 2 \: 3) = (1 \: 2 \: 3)(1 \: 2)(1 \: 2 \: 3) = (1 \: 2 \: 3)(1 \: 2)(1 \: 2 \: 3) = (1 \: 2 \: 3)(1 \: 2)(1 \: 2 \: 3) = (1 \: 2 \: 3)(1 \: 2)(1 \: 2 \: 3) = (1 \: 2 \: 3)(1 \: 2)(1 \: 2 \: 3) = (1 \: 2 \: 3)(1 \: 2)(1 \: 2 \: 3) = (1 \: 2 \: 3)(1 \: 2)(1 \: 2 \: 3) = (1 \: 2 \: 3)(1 \: 2)(1 \: 2 \: 3) = (1 \: 2 \: 3)(1 \: 2)(1 \: 2 \: 3) = (1 \: 2 \: 3)(1 \: 2)(1 \: 2 \: 3) = (1 \: 2 \: 3)(1 \: 2)(1 \: 2 \: 3) = (1 \: 2 \: 3)(1 \: 2)(1 \: 2 \: 3) = (1 \: 2 \: 3)(1 \: 2)(1 \: 2 \: 3) = (1 \: 2 \: 3)(1 \: 2)(1 \: 2 \: 3) = (1 \: 2 \: 3)(1 \: 2)(1 \: 2 \: 3) = (1 \: 2 \: 3)(1 \: 2)(1 \: 2 \: 3) = (1 \: 2 \: 3)(1 \: 2)(1 \: 2 \: 3) = (1 \: 2 \: 3)(1 \: 2)(1 \: 2 \: 3) = (1 \: 2 \: 3)(1 \: 2)(1 \: 2 \: 3) = (1 \: 2 \: 3)(1 \: 2)(1 \: 2 \: 3) = (1 \: 2 \: 3)(1 \: 2)(1 \: 2 \: 3) = (1 \: 2 \: 3)(1 \: 2)(1 \: 2 \: 3) = (1 \: 2 \: 3)(1 \: 2)(1 \: 2 \: 3) = (1 \: 2 \: 3)(1 \: 2)(1 \: 2 \: 3) = (1 \: 2 \: 3)(1 \: 2)(1 \: 2 \: 3) = (1 \: 2 \: 3)(1 \: 2)(1 \: 2 \: 3) = (1 \: 2 \: 3)(1 \: 2)(1 \: 2 \: 3) = (1 \: 2 \: 3)(1 \: 2)(1 \: 2 \: 3) = (1 \: 2 \: 3)(1 \: 2)(1 \: 2 \: 3) = (1 \: 2 \: 3)(1 \: 2)(1 \: 2 \: 3) = (1 \: 2 \: 3)(1 \: 2)(1 \: 2 \: 3) = (1 \: 2 \: 3)(1 \: 2)(1 \: 2 \: 3) = (1 \: 2 \: 3)(1 \: 2)(1 \: 2 \: 3) = (1 \: 2 \: 3)(1 \: 2)(1 \: 2 \: 3) = (1 \: 2 \: 3)(1 \: 2)(1 \: 2 \: 3) = (1 \: 2 \: 3)(1 \: 2)(1 \: 2 \: 3) = (1 \: 2 \: 3)(1 \: 2)(1 \: 2 \: 3) = (1 \: 2 \: 3)(1 \: 2)(1 \: 2 \: 3) = (1 \: 2 \: 3)(1 \: 2)(1 \: 2 \: 3) = (1 \: 2 \: 3)(1 \: 2)(1 \: 2 \: 3) = (1 \: 2 \: 3)(1 \: 2)(1 \: 2 \: 3) = (1 \: 2 \: 3)(1 \: 2)(1 \: 2 \: 3) = (1 \: 2 \: 3)(1 \: 2)(1 \: 2 \: 3) = (1 \: 2 \: 3)(1 \: 2)(1 \: 2 \: 3) = (1 \: 2 \: 3)(1 \: 2)(1 \: 2 \: 3) = (1 \: 2 \: 3)(1 \: 2)(1 \: 2 \: 3) = (1 \: 2 \: 3)(1 \: 2)(1 \: 2 \: 3) = (1 \: 2 \: 3)(1 \: 2)(1 \: 2 \: 3) = (1 \: 2 \: 3)(1 \: 2)(1 \: 2 \: 3) = (1 \: 2 \: 3)(1 \: 2)(1 \: 2 \: 3) = (1 \: 2 \: 3)(1 \: 2)(1 \: 2 \: 3) = (1 \: 2 \: 3)(1 \: 2)(1 \: 2 \: 3) = (1 \: 2 \: 3)(1 \: 2)(1 \: 2 \: 3) = (1 \: 2 \: 3)(1 \: 2)(1 \: