To construct a smooth convex function \( f \) that satisfies the given conditions, we need to ensure that \( f \) is continuous and differentiable at the points where the pieces of the function meet, specifically at \( r = \frac{\eta}{2} \) and \( r = \eta \). Additionally, the function must be convex.

Given:
- \( f(r) = \frac{1}{2} - \frac{e}{2}r \) for \( r \in ]-\frac{\eta}{2}, \frac{\eta}{2}[\)
- \( f(r) = a - r \) for \( r \in ]\eta, a[\)

We need to find a smooth transition between these two pieces at \( r = \frac{\eta}{2} \) and \( r = \eta \).

### Step 1: Define the function on the intervals

For \( r \in ]-\frac{\eta}{2}, \frac{\eta}{2}[\):
\[ f(r) = \frac{1}{2} - \frac{e}{2}r \]

For \( r \in ]\eta, a[\):
\[ f(r) = a - r \]

### Step 2: Ensure continuity at \( r = \frac{\eta}{2} \)

At \( r = \frac{\eta}{2} \), both pieces of the function must have the same value:
\[ f\left(\frac{\eta}{2}\right) = \frac{1}{2} - \frac{e}{2} \cdot \frac{\eta}{2} = \frac{1}{2} - \frac{e\eta}{4} \]
\[ f\left(\frac{\eta}{2}\right) = a - \frac{\eta}{2} \]

Equating these, we get:
\[ \frac{1}{2} - \frac{e\eta}{4} = a - \frac{\eta}{2} \]
Solving for \( a \):
\[ a = \frac{1}{2} + \frac{\eta}{2} - \frac{e\eta}{4} \]

### Step 3: Ensure continuity at \( r = \eta \)

At \( r = \eta \), both pieces of the function must have the same value:
\[ f(\eta) = \frac{1}{2} - \frac{e}{2} \cdot \eta = \frac{1}{2} - \frac{e\eta}{2} \]
\[ f(\eta) = a - \eta \]

Equating these, we get:
\[ \frac{1}{2} - \frac{e\eta}{2} = a - \eta \]
Substituting \( a = \frac{1}{2} + \frac{\eta}{2} - \frac{e\eta}{4} \):
\[ \frac{1}{2} - \frac{e\eta}{2} = \left( \frac{1}{2} + \frac{\eta}{2} - \frac{e\eta}{4} \right) - \eta \]
Simplifying:
\[ \frac{1}{2} - \frac{e\eta}{2} = \frac{1}{2} + \frac{\eta}{2} - \frac{e\eta}{4} - \eta \]
\[ -\frac{e\eta}{2} = \frac{\eta}{2} - \eta - \frac{e\eta}{4} \]
\[ -\frac{e\eta}{2} = \frac{\eta}{2} - \frac{2\eta}{2} - \frac{e\eta}{4} \]
\[ -\frac{e\eta}{2} = -\frac{\eta}{2} - \frac{e\eta}{4} \]
Multiplying through by 4 to clear the denominators:
\[ -2e\eta = -2\eta - e\eta \]
\[ -2e\eta + e\eta = -2\eta \]
\[ -e\eta = -2\eta \]
\[ e = 2 \]

### Step 4: Ensure smoothness (differentiability) at \( r = \frac{\eta}{2} \) and \( r = \eta \)

The derivative of \( f(r) \) for \( r \in ]-\frac{\eta}{2}, \frac{\eta}{2}[\) is:
\[ f'(r) = -\frac{e}{2} = -1 \]

The derivative of \( f(r) \) for \( r \in ]\eta, a[\) is:
\[ f'(r) = -1 \]

Since both derivatives are equal at \( r = \frac{\eta}{2} \) and \( r = \eta \), the function is smooth at these points.

### Final Function

Given \( e = 2 \), we have:
\[ a = \frac{1}{2} + \frac{\eta}{2} - \frac{2\eta}{4} = \frac{1}{2} + \frac{\eta}{2} - \frac{\eta}{2} = \frac{1}{2} \]

Thus, the function is:
\[ f(r) = \begin{cases} 
\frac{1}{2} - r & \text{if } r \in ]-\frac{\eta}{2}, \frac{\eta}{2}[] \\
a - r & \text{if } r \in ]\eta, a[
\end{cases} \]

Where \( a = \frac{1}{2} \).

Therefore, the final form of the function is:
\[ f(r) = \begin{cases} 
\frac{1}{2} - r & \text{if } r \in ]-\frac{\eta}{2}, \frac{\eta}{2}[] \\
\frac{1}{2} - r & \text{if } r \in ]\eta, a[
\end{cases} \]